New type for theta. A few admits to go to show it is a monad morphism

newio/DM.fst
@@ -60,14 +60,20 @@ let rec lemma_return_of_implies_exists_trace_of (x:'a) (m:io 'a) :
     end
   end
 
+unfold let io_wps (cmd:io_cmds) (arg:io_args cmd) : hist #event (io_resm cmd) = fun p h ->
+  match cmd with
+ // | GetTrace -> p [] h
+  | _ -> io_pre cmd arg h /\ (forall r. p [convert_call_to_event cmd arg r] r)
+
+let tret_of (m:free 'op 's 'a) : Type = (x:'a{x `return_of` m})
+
 (** Inspierd from Kenji's thesis (2.4.5) **)
-let rec theta #a
-  (m : io a) : hist a =
+let rec theta (#a:Type) (m : io a) : hist #event (x:a{x `return_of` m}) =
   match m with
   | Return x -> hist_return x
   | Call cmd arg k ->
-    hist_bind (io_wps cmd arg) (fun r -> theta (k r))
-  
+    hist_bind (io_resm cmd) (x:a{x `return_of` m}) (io_wps cmd arg) (fun r -> theta (k r))
+
 let rec lemma_theta_result_implies_post m p h : 
   Lemma 
     (requires theta m p h) 
@@ -80,19 +86,54 @@ let rec lemma_theta_result_implies_post m p h :
         let e::klt = lt in
         let (| cmd', arg', res' |) = destruct_event e in
         lemma_theta_result_implies_post (k res') (hist_post_shift p [convert_call_to_event cmd arg res']) (convert_call_to_event cmd arg res' :: h);
-        assert (trace_of klt (k res') x);
-        assert (hist_post_shift p [convert_call_to_event cmd arg res'] klt x)
+        assert (trace_of klt (k res') x) by (smt ());
+        assert (hist_post_shift p [convert_call_to_event cmd arg res'] klt x) by (smt ())
       end
     end
   end
 
+let rec lemma_return_of_free_bind (m:io 'a) (mx:'a{mx `return_of` m}) (f:(x:'a{x `return_of` m}) -> io 'b) :
+  Lemma (forall fx. fx `return_of` (f mx) ==> fx `return_of` (io_bind m f)) =
+  introduce forall fx. fx `return_of` (f mx) ==> fx `return_of` (io_bind m f) with begin
+    introduce fx `return_of` (f mx) ==> fx `return_of` (io_bind m f) with _. begin
+      match m with
+      | Return _ -> ()
+      | Call cmd arg k -> begin
+        eliminate exists r. return_of mx (k r) returns fx `return_of` (io_bind m f) with _. begin
+	  lemma_return_of_free_bind (k r) mx f
+	end
+      end
+    end
+  end
+
+unfold 
+let cast_hist_bind_return_of
+  (m:io 'a)
+  (mx:'a{mx `return_of` m})
+  (f:(x:'a{x `return_of` m}) -> io 'b)
+  (wp:hist (x:'b{x `return_of` f mx})) :
+  Tot (hist (x:'b{x `return_of` (io_bind m f)})) =
+  lemma_return_of_free_bind m mx f;
+  wp
+
+let theta_of_f_x 
+  (m:io 'a)
+  (f:(x:'a{x `return_of` m}) -> io 'b)
+  (mx:'a{mx `return_of` m}) :
+  Tot (hist (x:'b{x `return_of` (io_bind m f)})) =
+  cast_hist_bind_return_of m mx f (theta (f mx))
+
+(**
+let hist_bind' (m:io 'a) (f:'a -> io 'b) (wp1:hist (x:'a{x `return_of` m})) (wp2:((x:'a) -> hist (x':'b{x' `return_of` (f x)}))) : hist (x:'b{x `return_of` io_bind m f})=
+  hist_bind wp1 wp2**)
+  
 let lemma_theta_is_monad_morphism_ret v h p :
   Lemma (theta (io_return v) == hist_return v) by (compute ()) = ()
 
 (** TODO: remove the admits **)
-let rec lemma_theta_is_monad_morphism_bind (m:io 'a) (f:(x:'a) -> io 'b) :
+let rec lemma_theta_is_monad_morphism_bind (m:io 'a) (f:(x:'a{x `return_of` m}) -> io 'b) :
   Lemma
-    (theta (io_bind m f) == hist_bind (theta m) (fun x -> theta (f x))) = 
+    (theta (io_bind m f) == hist_bind _ _ (theta m) (theta_of_f_x m f)) = 
   match m with
   | Return x ->
     calc (==) {
@@ -102,16 +143,19 @@ let rec lemma_theta_is_monad_morphism_bind (m:io 'a) (f:(x:'a) -> io 'b) :
       == {} // unfold io_bind
       theta (f x); 
       == { _ by (tadmit ()) } // unfold hist_bind
-      hist_bind (hist_return x) (fun x -> theta (f x));
+      hist_bind _ _ (hist_return x) (theta_of_f_x m f);
       == { _ by (compute ()) } // unfold theta
-      hist_bind (theta (Return x)) (fun x -> theta (f x));
+      hist_bind _ _ (theta (Return x)) (theta_of_f_x m f);
     };
     (** this should be inside calc, but for some reason it fails there **)
-    assert (hist_bind (theta (Return x)) (fun x -> theta (f x))
-      == hist_bind (theta m) (fun x -> theta (f x))) by (rewrite_eqs_from_context ())
+    assert (hist_bind _ _ (theta (Return x))  (theta_of_f_x m f)
+      == hist_bind _ _ (theta m) (theta_of_f_x m f)) by (rewrite_eqs_from_context ())
   | Call cmd arg k ->
+
+    admit ()
+     (**
     (** this should be useful later to do a rewrite **)
-    introduce forall (r:io_resm cmd). theta (io_bind (k r) f) == hist_bind (theta (k r)) (fun x -> theta (f x)) with begin
+    introduce forall (r:io_resm cmd). theta (io_bind (k r) f) == hist_bind (theta (k r)) (theta_of_f_x m f) with begin
       lemma_theta_is_monad_morphism_bind (k r) f
     end;
 
@@ -120,19 +164,19 @@ let rec lemma_theta_is_monad_morphism_bind (m:io 'a) (f:(x:'a) -> io 'b) :
       == {}
       theta (io_bind (Call cmd arg k) f);
       == { _ by (compute ()) } // unfold io_bind
-      theta (Call cmd arg (fun r -> io_bind (k r) f));
-      == { _ by (compute ()) } // unfold theta
+      theta (Call cmd arg (fun r -> io_bind (k r) f)) <: hist (x:'b{x `return_of` Call cmd arg (fun r -> io_bind (k r) f)});
+      == { _ by (tadmit (); (); dump "h") } // unfold theta
       hist_bind (io_wps cmd arg) (fun r -> theta (io_bind (k r) f));
       == { _ by (tadmit ()) } // rewrite here by applying this lemma again for (k r) and f
-      hist_bind (io_wps cmd arg) (fun r -> hist_bind (theta (k r)) (fun x -> theta (f x)));
-      == { lemma_hist_bind_associativity (io_wps cmd arg) (fun r -> theta (k r)) (fun x -> theta (f x)) }
-      hist_bind (hist_bind (io_wps cmd arg) (fun r -> theta (k r))) (fun x -> theta (f x));
+      hist_bind (io_wps cmd arg) (fun r -> hist_bind (theta (k r)) (theta_of_f_x m f));
+      == { lemma_hist_bind_associativity (io_wps cmd arg) (fun r -> theta (k r)) (theta_of_f_x m f) }
+      hist_bind #_ #(x:'a{x `return_of` m}) #(x:'b{x `return_of` io_bind m f}) (hist_bind (io_wps cmd arg) (fun r -> theta (k r))) (theta_of_f_x m f);
       == { _ by (compute ()) } // unfold theta
-      hist_bind (theta (Call cmd arg k)) (fun x -> theta (f x));
+      hist_bind #_ #(x:'a{x `return_of` m}) #(x:'b{x `return_of` io_bind m f}) (theta (Call cmd arg k)) (theta_of_f_x m f);
     };
     (** this should be inside calc, but for some reason it fails there **)
-    assert (hist_bind (theta (Call cmd arg k)) (fun x -> theta (f x))
-      == hist_bind (theta m) (fun x -> theta (f x))) by (rewrite_eqs_from_context ())
+    assert (hist_bind (theta (Call cmd arg k)) (theta_of_f_x m f)
+      == hist_bind (theta m) (theta_of_f_x m f)) by (rewrite_eqs_from_context ()) **)
 
 // The Dijkstra Monad
 let dm (a:Type) (wp:hist a) =
@@ -141,19 +185,54 @@ let dm (a:Type) (wp:hist a) =
 let dm_return (a : Type) (x : a) : dm a (hist_return x) =
   io_return x
 
+let awesome_lemma 
+  (a b:Type)
+  (v:io a)
+  (f:(x:a{x `return_of` v}) -> io b) : 
+  Lemma (
+  (hist_bind (x:a{x `return_of` v}) b (theta v) (fun x -> theta (f x))) == 
+    ((hist_bind (x:a{x `return_of` v}) (x:b{x `return_of` io_bind v f}) (theta v) (theta_of_f_x v f)) <: hist b)) by 
+    (explode ();
+     tadmit (); tadmit ();
+    ExtraTactics.rewrite_lemma 5 6;
+    norm [delta_only [`%theta_of_f_x; `%cast_hist_bind_return_of]];
+    tadmit ();
+    dump "H")= () 
+    
 let dm_bind
   (a b : Type)
   (wp_v : hist a)
   (wp_f: a -> hist b)
   (v : dm a wp_v)
   (f : (x:a{x `return_of` v} -> dm b (wp_f x))) :
-  Tot (dm b (hist_bind wp_v wp_f)) =
+  Tot (dm b (hist_bind _ _ wp_v wp_f)) =
   (** we lost the fact that theta is a monad morphism because we added
       the refinement `return_of` on the free_bind. We can prove this bind, 
       if we specialize the proof (Theo was able to that for his DM), but that
       implies that we do not get a DM for free. **)
-  // lemma_theta_is_monad_morphism_bind v f;
-  admit ();
+  
+  (** hist is monotonic. **)
+  
+  lemma_theta_is_monad_morphism_bind v f;
+  (**
+  calc (==) {
+    theta (io_bind v f);
+    == { lemma_theta_is_monad_morphism_bind v f }
+    hist_bind (x:a{x `return_of` v}) _ (theta v) (theta_of_f_x v f);
+    == { _ by (norm [delta_only [`%theta_of_f_x; `%cast_hist_bind_return_of]]; dump "H") }
+    hist_bind (x:a{x `return_of` v}) b (theta v) (fun x -> theta (f x));
+  }; **)
+  assert (theta (io_bind v f) == hist_bind (x:a{return_of x v}) (x:b{return_of x (io_bind v f)}) (theta v) (theta_of_f_x v f)); 
+  assert (wp_v `hist_ord` theta v);
+  assert (forall (x:a{x `return_of` v}). wp_f x `hist_ord #_ #b` theta (f x));
+
+  assert (hist_bind a b wp_v wp_f `hist_ord #_ #b`
+  	   hist_bind (x:a{x `return_of` v}) _ (theta v) (fun x -> theta (f x)));
+	   
+  awesome_lemma a b v f;
+  (** goal: **)
+  assert (hist_bind _ b wp_v wp_f `hist_ord #_ #b` theta (io_bind v f));
+
   io_bind v f
 
 let dm_subcomp (a:Type) (wp1 wp2: hist a) (f : dm a wp1) :
@@ -169,7 +248,7 @@ let lemma_hist_bind_implies_wp2_if_x
   (wp1:hist 'a) (wp2:'a -> hist 'b)
   (m:dm 'a wp1) p h x :
   Lemma 
-    (requires (hist_bind wp1 wp2 p h /\ x `return_of` m))
+    (requires (hist_bind _ _ wp1 wp2 p h /\ x `return_of` m))
     (ensures (exists lt. wp2 x (hist_post_shift p lt) (List.rev lt @ h))) =
   lemma_theta_result_implies_post m (fun lt r -> wp2 r (hist_post_shift p lt) (rev lt @ h)) h;
   lemma_return_of_implies_exists_trace_of x m
