newio/Hist.fst
@@ -15,41 +15,42 @@ The history is in reverse chronological order.
 At the end of an io computation, the local trace is
 reversed and appended to the history. **)
 
-let hist_post (#event) a = lt:list event -> r:a -> Type0
-let hist_pre (#event) = h:list event -> Type0
+let hist_post (#event:Type) a = lt:list event -> r:a -> Type0
+let hist_pre (#event:Type) = h:list event -> Type0
 
-private let hist0 (#event) a = hist_post #event a -> hist_pre #event
+private let hist0 (#event:Type) a = hist_post #event a -> hist_pre #event
 
 unfold
-let hist_post_ord (p1 p2:hist_post 'a) = forall lt r. p1 lt r ==> p2 lt r
+let hist_post_ord (#event:Type) (p1 p2:hist_post #event 'a) = forall lt r. p1 lt r ==> p2 lt r
 
-let hist_wp_monotonic (wp:hist0 'a) =
+let hist_wp_monotonic (#event:Type) (wp:hist0 #event 'a) =
   forall p1 p2. (p1 `hist_post_ord` p2) ==> (forall h. wp p1 h ==> wp p2 h)
 
 let hist #event a = wp:(hist0 #event a){hist_wp_monotonic wp}
 
-let hist_return (x:'a) : hist 'a =
+let hist_return (#event:Type) (x:'a) : hist #event 'a =
   fun p _ -> p [] x
 
 unfold
-let hist_post_shift (p:hist_post 'a) (lt:list 'event) : hist_post 'a =
+let hist_post_shift (#event:Type) (p:hist_post #event 'a) (lt:list event) : hist_post #event 'a =
   fun lt' r -> p (lt @ lt') r
 
 unfold
 let hist_post_bind
-  (h:list 'event)
-  (kw : 'a -> hist 'b)
-  (p:hist_post 'b) :
-  Tot (hist_post 'a) =
+  (#event:Type)
+  (h:list event)
+  (kw : 'a -> hist #event 'b)
+  (p:hist_post #event 'b) :
+  Tot (hist_post #event 'a) =
   fun lt r ->
     kw r (hist_post_shift p lt) (List.rev lt @ h)
 
 unfold
-let hist_bind (w : hist 'a) (kw : 'a -> hist 'b) : hist 'b =
-  fun p h -> w (hist_post_bind h kw p) h
+let hist_bind (#event:Type) (a b:Type) (w : hist #event a) (kw : a -> hist #event b) : hist #event b =
+  fun p h -> w (hist_post_bind #a #b #event h kw p) h
 
 unfold
-let wp_lift_pure_hist (w : pure_wp 'a) : hist 'a =
+let wp_lift_pure_hist (#event:Type) (w : pure_wp 'a) : hist #event 'a =
   FStar.Monotonic.Pure.elim_pure_wp_monotonicity_forall ();
   fun p _ -> w (p [])
 
@@ -64,11 +65,11 @@ val hist_ord (#event:Type) (#a : Type) : hist #event a -> hist #event a -> Type0
 let hist_ord wp1 wp2 = forall h p. wp1 p h ==> wp2 p h
 
 unfold
-let hist_if_then_else (wp1 wp2:hist 'a) (b:bool) : hist 'a =
+let hist_if_then_else (wp1 wp2:hist #'event 'a) (b:bool) : hist #'event 'a =
   fun p h -> (b ==> wp1 p h) /\ ((~b) ==> wp2 p h)
   
 let lemma_hist_bind_associativity (w1:hist 'a) (w2:'a -> hist 'b) (w3: 'b -> hist 'c) :
   Lemma (
-    hist_bind w1 (fun r1 -> hist_bind (w2 r1) w3) == hist_bind (hist_bind w1 w2) w3)
+    hist_bind _ _ w1 (fun r1 -> hist_bind  _ _ (w2 r1) w3) == hist_bind _ _ (hist_bind _ _ w1 w2) w3)
   by (l_to_r [`List.Tot.Properties.rev_append;`List.Tot.Properties.append_assoc]) =
   () 
